core/Tactics.v
@@ -143,17 +143,28 @@ Ltac inv_implicit_return :=
 
 Ltac start_function :=
   lazymatch goal with
-  | |- hoare_func _ _ _ _ _ ?post =>
-      eapply hoare_func_internal';
-        [ reflexivity (* length (filter_in params) = length pre_arg *)
-        | reflexivity (* is_no_dup *)
-        | reflexivity (* eval_write_vars *)
-        | idtac (* hoare_block *)
-        | inv_func_copy_out (* inv_func_copy_out *)
-        | inv_implicit_return
-        ]
-  | _ => fail "The goal is not in the form of (hoare_func _ _ (ARG _ (MEM _ (EXT _))) _ _"
-    "(EX ... ARG_RET _ (MEM _ (EXT _)))"
+  | |- fundef_satisfies_spec _ _ _ ?spec =>
+      try unfold spec;
+      repeat lazymatch goal with
+      | |- fundef_satisfies_spec _ _ _ (fs_bind (fun x => _)) =>
+        intro x
+      end;
+      split; [idtac | admit];
+      (* handle hoare_func *)
+      lazymatch goal with
+      | |- hoare_func _ _ _ _ _ ?post =>
+        eapply hoare_func_internal';
+          [ reflexivity (* length (filter_in params) = length pre_arg *)
+          | reflexivity (* is_no_dup *)
+          | reflexivity (* eval_write_vars *)
+          | idtac (* hoare_block *)
+          | inv_func_copy_out (* inv_func_copy_out *)
+          | inv_implicit_return
+          ]
+      | _ => fail "The goal is not in the form of (hoare_func _ _ (ARG _ (MEM _ (EXT _))) _ _"
+               "(EX ... ARG_RET _ (MEM _ (EXT _)))"
+      end
+  | _ => fail "The goal is not in the form of (fundef_satisfies_spec _ _ _)"
   end.
 
 Ltac forward_call_func func_spec :=
